bytestring: split core out

theories/prelude/bytestring.v
@@ -3,11 +3,12 @@
  * This software is distributed under the terms of the BedRock Open-Source License.
  * See the LICENSE-BedRock file in the repository root for details.
  *)
-Require Import Coq.Structures.OrderedType.
 From stdpp Require Import countable strings namespaces.
+Require Export bedrock.prelude.bytestring_core.
 
 #[local] Set Default Proof Using "Type".
 
+(** Bytestring extensions. Integrate with stdpp and strings. *)
 (** bytes *)
 Instance byte_inhabited : Inhabited Byte.byte := populate Byte.x00.
 Instance byte_eq_dec : EqDecision Byte.byte := Byte.byte_eq_dec.
@@ -21,86 +22,15 @@ Proof.
   abstract (by intros []).
 Defined.
 
-Definition byte_parse (b : Byte.byte) : Byte.byte := b.
-Definition byte_print (b : Byte.byte) : Byte.byte := b.
+Instance bytestring_eq_dec : EqDecision bs := BS.eq_dec.
 
-(** comparison *)
-Definition byte_cmp (a b : Byte.byte) : comparison :=
-  N.compare (Byte.to_N a) (Byte.to_N b).
-
-Delimit Scope byte_scope with byte.
-String Notation Byte.byte byte_parse byte_print : byte_scope.
-
-Bind Scope byte_scope with Byte.byte.
-
-Lemma byte_cmp_refl a : byte_cmp a a = Eq.
-Proof. intros. apply N.compare_refl. Qed.
-
-Lemma byte_to_N_inj x y : Byte.to_N x = Byte.to_N y <-> x = y.
+Instance bytestring_inhabited : Inhabited bs := populate ""%bs.
+Instance bytestring_countable : Countable bs.
 Proof.
-  split. 2: now intros ->.
-  intros Heq.
-  enough (Some x = Some y) as [= ->] by easy.
-  do 2 rewrite <- Byte.of_to_N.
-  now rewrite Heq.
-Qed.
+  apply (inj_countable' BS.print BS.parse),
+    BS.print_parse_inv.
+Defined.
 
-Module OT_byte <: OrderedType.OrderedType with Definition t := Byte.byte.
-  Definition t := Byte.byte.
-  Definition eq := fun l r => byte_cmp l r = Eq.
-  Definition lt := fun l r => byte_cmp l r = Lt.
-  Theorem eq_refl (x : t) : eq x x.
-  Proof.
-    intros; apply N.compare_refl.
-  Qed.
-  Theorem eq_sym (x y : t) : eq x y -> eq y x.
-  Proof.
-    intros Hxy. eapply N.compare_eq in Hxy. unfold eq, byte_cmp.
-    rewrite Hxy. apply eq_refl.
-  Qed.
-  Theorem eq_trans (x y z : t) : eq x y -> eq y z -> eq x z.
-  Proof.
-    intros Hxy Hyz. eapply N.compare_eq in Hxy. eapply N.compare_eq in Hyz.
-    unfold eq, byte_cmp. rewrite -> Hxy, Hyz.
-    apply eq_refl.
-  Qed.
-  Theorem lt_trans (x y z : t) : lt x y -> lt y z -> lt x z.
-  Proof.
-    unfold lt, byte_cmp. rewrite ->!N.compare_lt_iff.
-    lia.
-  Qed.
-  Theorem lt_not_eq (x y : t) : lt x y -> ~ eq x y.
-  Proof.
-    unfold lt, eq, byte_cmp. rewrite ->N.compare_lt_iff, N.compare_eq_iff.
-    lia.
-  Qed.
-  Definition compare (x y : t) : OrderedType.Compare lt eq x y.
-  Proof.
-    refine (match byte_cmp x y as X return byte_cmp x y = X -> OrderedType.Compare lt eq x y with
-      | Eq => fun pf => OrderedType.EQ pf
-      | Lt => fun pf => OrderedType.LT pf
-      | Gt => fun pf => OrderedType.GT _
-      end Logic.eq_refl).
-    unfold lt, byte_cmp.
-    abstract (rewrite N.compare_antisym; apply CompOpp_iff, pf).
-  Defined.
-
-  Definition eq_dec (x y : t) : {eq x y} + {~ eq x y}.
-  Proof.
-    refine (match byte_cmp x y as Z return byte_cmp x y = Z -> _ with
-        | Eq => fun pf => left pf
-        | _ => fun _ => right _
-        end Logic.eq_refl);
-    abstract congruence.
-  Defined.
-End OT_byte.
-
-Theorem byte_cmp_spec x y : CompareSpec (x = y) (OT_byte.lt x y) (OT_byte.lt y x) (byte_cmp x y).
-Proof.
-  unfold byte_cmp, OT_byte.lt, byte_cmp.
-  destruct (N.compare_spec (Byte.to_N x) (Byte.to_N y)); constructor; auto.
-  apply byte_to_N_inj. assumption.
-Qed.
 
 (** bytestrings *)
 (** Many functions on byte strings are meant to be always used
@@ -109,76 +39,13 @@ qualified, as they conflict with similar functions from [List] or [String].
 All such functions are collected in a module [BS], which is not meant
 to be imported, as it defines names like [t].
 *)
-
 Module Import BS.
-  Inductive t : Set :=
-  | EmptyString
-  | String (_ : Byte.byte) (_ : t).
-
-  Definition eq_dec (x y : t) : {x = y} + {x <> y}.
-  Proof. decide equality. apply Byte.byte_eq_dec. Defined.
-
-  Fixpoint print (b : t) : list Byte.byte :=
-    match b with
-    | EmptyString => nil
-    | String b bs => b :: print bs
-    end.
-
-  Fixpoint parse (b : list Byte.byte) : t :=
-    match b with
-    | nil => EmptyString
-    | b :: bs => String b (parse bs)
-    end.
-
-  Lemma print_parse_inv (x : BS.t) :
-    BS.parse (BS.print x) = x.
-  Proof.
-    induction x; simpl; intros; auto.
-    f_equal; auto.
-  Qed.
-
-  Lemma parse_print_inv (x : list Byte.byte) :
-    BS.print (BS.parse x) = x.
-  Proof.
-    induction x; simpl; intros; auto.
-    f_equal; auto.
-  Qed.
-
-  Instance t_dec : EqDecision t.
-  Proof. solve_decision. Defined.
-
-  (** Module [Bytestring_notations] is exported below, and contains
-  definitions that can be safely exported. *)
-  Module Import Bytestring_notations.
-    Definition bs := BS.t.
-
-    Declare Scope bs_scope.
-    Delimit Scope bs_scope with bs.
-    Bind Scope bs_scope with bs.
-
-    #[local] Fixpoint append (x y : bs) : bs :=
-      match x with
-      | BS.EmptyString => y
-      | BS.String x xs => BS.String x (append xs y)
-      end.
-
-    Notation "x ++ y" := (append x y) : bs_scope.
-
-    String Notation BS.t BS.parse BS.print : bs_scope.
-
-    Instance bytestring_inhabited : Inhabited bs := populate ""%bs.
-    Instance bytestring_countable : Countable bs.
-    Proof.
-      apply (inj_countable' BS.print BS.parse),
-        BS.print_parse_inv.
-    Defined.
-  End Bytestring_notations.
-  Notation append := Bytestring_notations.append.
+  Export bytestring_core.BS.
 
   Fixpoint to_string (b : bs) : string :=
     match b with
-    | EmptyString => String.EmptyString
-    | String x xs => String.String (Ascii.ascii_of_byte x) (to_string xs)
+    | BS.EmptyString => String.EmptyString
+    | BS.String x xs => String.String (Ascii.ascii_of_byte x) (to_string xs)
     end.
 
   Fixpoint of_string (b : string) : bs :=
@@ -205,175 +72,9 @@ Module Import BS.
     - by rewrite IHb', Ascii.ascii_of_byte_of_ascii.
   Qed.
 
-  Fixpoint rev (acc s : bs) : bs :=
-    match s with
-    | EmptyString => acc
-    | String s ss => rev (String s acc) ss
-    end.
-
-  Fixpoint prefix (s1 s2 : bs) {struct s1} : bool :=
-    match s1 with
-    | EmptyString => true
-    | String x xs =>
-      match s2 with
-      | EmptyString => false
-      | String y ys =>
-        if Byte.byte_eq_dec x y then prefix xs ys
-        else false
-      end
-    end%bs.
-
-  (** [substring n m s] returns the substring of [s] that starts
-      at position [n] and of length [m];
-      if this does not make sense it returns [""] *)
-  Fixpoint substring (n m : nat) (s : bs) : bs :=
-    match n, m, s with
-    | O,    O,    _              => BS.EmptyString
-    | O,    S m', BS.EmptyString => s
-    | O,    S m', BS.String c s' => BS.String c (substring 0 m' s')
-    | S n', _,    BS.EmptyString => s
-    | S n', _,    BS.String c s' => substring n' m s'
-    end.
-
-  Fixpoint index (n : nat) (s1 s2 : bs) {struct s2} : option nat :=
-    match s2 with
-    | EmptyString =>
-        match n with
-        | 0 => match s1 with
-              | "" => Some 0
-              | String _ _ => None
-              end
-        | S _ => None
-        end
-    | String _ s2' =>
-        match n with
-        | 0 =>
-            if prefix s1 s2
-            then Some 0
-            else match index 0 s1 s2' with
-                | Some n0 => Some (S n0)
-                | None => None
-                end
-        | S n' => match index n' s1 s2' with
-                  | Some n0 => Some (S n0)
-                  | None => None
-                  end
-        end
-    end%bs.
-
-  Fixpoint length (l : bs) : nat :=
-    match l with
-    | EmptyString => 0
-    | String _ l => S (length l)
-    end.
-
-  Lemma print_length (s : bs) :
-    List.length (BS.print s) = BS.length s.
-  Proof.
-    induction s; simpl.
-    - easy.
-    - now rewrite IHs.
-  Qed.
-
-  Fixpoint contains (start : nat) (keys : list bs) (fullname : bs) :bool :=
-    match keys with
-    | kh::ktl =>
-      match index start kh fullname with
-      | Some n => contains (n + length kh) ktl fullname
-      | None => false
-      end
-    | [] => true
-    end.
-
-  Definition eqb (a b : bs) : bool :=
-    if eq_dec a b then true else false.
-
-  #[deprecated(since="2021-09-21", note="Use [byte_to_N_inj]")]
-  Notation to_N_inj := byte_to_N_inj.
+  #[deprecated(since="2021-09-21", note="Use [decide (arg1 = arg2)]")]
+  Notation t_dec := bytestring_eq_dec.
 End BS.
-Export Bytestring_notations.
-
-Fixpoint bs_cmp (xs ys : bs) : comparison :=
-  match xs , ys with
-  | BS.EmptyString , BS.EmptyString => Eq
-  | BS.EmptyString , _ => Lt
-  | _ , BS.EmptyString => Gt
-  | BS.String x xs , BS.String y ys =>
-    match byte_cmp x y with
-    | Eq => bs_cmp xs ys
-    | x => x
-    end
-  end%bs.
-
-Module OT_bs <: OrderedType.OrderedType with Definition t := bs.
-  Definition t := bs.
-  Definition eq := @eq bs.
-  Definition lt := fun l r => bs_cmp l r = Lt.
-
-  Theorem lm x y : CompareSpec (x = y) (lt x y) (lt y x) (bs_cmp x y).
-  Proof.
-    revert y; induction x; destruct y; simpl.
-    - constructor; reflexivity.
-    - constructor. reflexivity.
-    - constructor. reflexivity.
-    - unfold lt; simpl.
-      destruct (byte_cmp_spec b b0); simpl.
-      + subst. destruct (IHx y); constructor; eauto.
-        congruence.
-        destruct (byte_cmp_spec b0 b0); try congruence.
-        red in H0. rewrite OT_byte.eq_refl in H0. congruence.
-      + constructor; auto.
-      + red in H. rewrite H. constructor; auto.
-  Qed.
-
-  Definition compare (x y : t) : OrderedType.Compare lt eq x y.
-  Proof.
-    refine (
-      match bs_cmp x y as X return bs_cmp x y = X -> OrderedType.Compare lt eq x y  with
-      | Eq => fun pf => OrderedType.EQ _
-      | Lt => fun pf => OrderedType.LT pf
-      | Gt => fun pf => OrderedType.GT _
-      end (Logic.eq_refl));
-    abstract (generalize (lm x y); rewrite pf; inversion 1; auto).
-  Defined.
-
-  Theorem eq_refl (x : t) : eq x x.
-  Proof. reflexivity. Qed.
-  Theorem eq_sym (x y : t) : eq x y -> eq y x.
-  Proof. eapply eq_sym. Qed.
-  Theorem eq_trans (x y z : t) : eq x y -> eq y z -> eq x z.
-  Proof. eapply eq_trans. Qed.
-  Theorem lt_trans (x y z : t) : lt x y -> lt y z -> lt x z.
-  Proof.
-    unfold lt.
-    revert y z.
-    induction x; destruct y; simpl; try congruence.
-    - destruct z; congruence.
-    - destruct (byte_cmp_spec b b0); subst.
-      + destruct z; auto.
-        destruct (byte_cmp b0 b); auto.
-        eauto.
-      + destruct z; auto.
-        red in H.
-        destruct (byte_cmp b0 b1) eqn:?.
-        * generalize (byte_cmp_spec b0 b1).
-          rewrite Heqc. inversion 1.
-          subst. rewrite H. auto.
-        * generalize (OT_byte.lt_trans _ _ _ H Heqc). unfold OT_byte.lt.
-          intro X; rewrite X. auto.
-        * congruence.
-      + congruence.
-  Qed.
-  Theorem lt_not_eq (x y : t) : lt x y -> ~ eq x y.
-  Proof.
-    unfold lt, eq.
-    intros Heq ->.
-    induction y; simpl in *; try congruence.
-    rewrite ->byte_cmp_refl in Heq. auto.
-  Qed.
-
-  Definition eq_dec := BS.eq_dec.
-End OT_bs.
 
 (* stdpp-specific. *)
 Notation "N .@@ x" := (ndot (A := bs) N x%bs)
